Computability/test.lean
@@ -117,8 +117,6 @@ def c_le_guard  (c:Code) := (c_bind_opt (c.comp right)).comp (c_if_le_te.comp₄
 section pair_g
 namespace Nat.RecursiveIn.Code
 
---
--- def c_pair_g : Code→Code→Code := fun cf cg => (c_bind_opt2 pair).comp (pair cf cg)
 -- input is of the form (s,x)
 def c_pair_g : Code→Code→Code := fun cf cg =>
   let x         := right
@@ -127,9 +125,9 @@ def c_pair_g : Code→Code→Code := fun cf cg =>
   c_if_le_te.comp₄ x s
 
   (
-    c_ifz.comp₂ ( cf.comp c_id) $ pair (c_const 0) $
-    c_ifz.comp₂ ( cg.comp c_id) $ pair (c_const 0) $
-    succ.comp (pair (c_pred.comp ( cf.comp c_id)) (c_pred.comp ( cg.comp c_id)))
+    c_ifz.comp₃ (cf.comp c_id) (c_const 0) $
+    c_ifz.comp₃ (cg.comp c_id) (c_const 0) $
+    succ.comp (pair (c_pred.comp (cf.comp c_id)) (c_pred.comp (cg.comp c_id)))
   )
 
   (c_const 0)
@@ -140,7 +138,7 @@ def c_pair_g : Code→Code→Code := fun cf cg =>
   let x         := inp.r
   let s         := inp.l
   Encodable.encode (do guard (x≤s); Nat.pair <$> ((@Denumerable.ofNat (Option ℕ)) (eval_prim O cf inp)) <*> ((@Denumerable.ofNat (Option ℕ)) (eval_prim O cg inp))) := by
-  
+
   lift_lets
   extract_lets
   expose_names
@@ -163,7 +161,7 @@ def c_pair_g : Code→Code→Code := fun cf cg =>
     simp [x_1, x]
   have hs : eval_prim O s_1 inp = s := by
     simp [s_1, s]
-  
+
 
   cases Classical.em (x≤s) with
   | inl hl =>
@@ -197,6 +195,88 @@ def c_pair_g : Code→Code→Code := fun cf cg =>
 -- @[simp] theorem c_pair_g_ev :eval O (c_pair_g) = fun (n:ℕ) => Encodable.encode (do guard (n.r≤n.l); Nat.pair <$> evaln O (k + 1) cf n <*> evaln O (k + 1) cg n : Option ℕ) := by rw [← eval_prim_eq_eval (c_pair_g_ev_pr)]; simp only [c_pair_g_evp]
 end Nat.RecursiveIn.Code
 end pair_g
+
+section comp_g
+namespace Nat.RecursiveIn.Code
+
+-- input is of the form (s,x)
+def c_comp_g : Code→Code→Code := fun cf cg =>
+  let x         := right
+  let s         := left
+
+  c_if_le_te.comp₄ x s
+
+  (
+    c_ifz.comp₃ (cg.comp c_id) (c_const 0) $
+    c_ifz.comp₃ (cf.comp c_id) (c_const 0) $
+    succ.comp (pair (c_pred.comp (cf.comp c_id)) (c_pred.comp (cg.comp c_id)))
+  )
+
+  (c_const 0)
+@[simp] theorem c_comp_g_ev_pr (hcf:code_prim cf) (hcg:code_prim cg):code_prim (c_comp_g cf cg) := by
+  unfold c_comp_g
+  repeat (first|assumption|simp|constructor)
+@[simp] theorem c_comp_g_evp:eval_prim O (c_comp_g cf cg) inp =
+  let x         := inp.r
+  let s         := inp.l
+  Encodable.encode (do guard (x≤s); Nat.pair <$> ((@Denumerable.ofNat (Option ℕ)) (eval_prim O cf inp)) <*> ((@Denumerable.ofNat (Option ℕ)) (eval_prim O cg inp))) := by
+
+  lift_lets
+  extract_lets
+  expose_names
+
+  simp only [Option.bind_eq_bind]
+  simp [Encodable.encode]
+  simp [Seq.seq]
+
+  unfold c_comp_g
+  lift_lets
+  extract_lets
+  expose_names
+  simp [eval_prim]
+  have h0 : (Denumerable.ofNat (Option ℕ) 0) = Option.none := by exact rfl
+  have h1 {x} (h2:¬x=0) : x=x-1+1 := by exact Eq.symm (succ_pred_eq_of_ne_zero h2)
+  have h2 {x} (h3:¬x=0) : (Denumerable.ofNat (Option ℕ) x) = Option.some (x-1) := by
+    rw (config := {occs := .pos [1]}) [h1 h3]
+    exact rfl
+  have hx : eval_prim O x_1 inp = x := by
+    simp [x_1, x]
+  have hs : eval_prim O s_1 inp = s := by
+    simp [s_1, s]
+
+
+  cases Classical.em (x≤s) with
+  | inl hl =>
+    simp [hl]
+    cases Classical.em ((eval_prim O cf inp)=0) with
+    | inl hll => simp [hll, h0]
+    | inr hlr =>
+      simp [hlr, h2 hlr]
+      cases Classical.em ((eval_prim O cg inp)=0) with
+      | inl hlrl => simp [hlrl, h0]
+      | inr hlrr =>
+        simp [hlrr, h2 hlrr]
+        simp [hx,hs]
+        simp [hl]
+
+  | inr hr =>
+    simp [hr]
+    cases Classical.em ((eval_prim O cf inp)=0) with
+    | inl hrl => simp [hrl, h0]
+    | inr hrr =>
+      simp [hrr, h2 hrr]
+      cases Classical.em ((eval_prim O cg inp)=0) with
+      | inl hrrl => simp [hrrl, h0]
+      | inr hrrr =>
+        simp [hrrr, h2 hrrr]
+        simp [Option.bind]
+        simp [hx,hs]
+        apply gt_of_not_le hr
+
+
+-- @[simp] theorem c_comp_g_ev :eval O (c_comp_g) = fun (n:ℕ) => Encodable.encode (do guard (n.r≤n.l); Nat.pair <$> evaln O (k + 1) cf n <*> evaln O (k + 1) cg n : Option ℕ) := by rw [← eval_prim_eq_eval (c_comp_g_ev_pr)]; simp only [c_comp_g_evp]
+end Nat.RecursiveIn.Code
+end comp_g
 
 
 
@@ -292,6 +372,69 @@ theorem pair_nonzero_right_pos_aux : ¬ (Nat.pair x (s+1)=0) := by
 
 
 
+def evaln' (O:ℕ→ℕ) : ℕ → Code → ℕ → Option ℕ :=
+  fun s code n => do
+  guard (n ≤ s-1)
+  match s, code with
+  | 0, _ => Option.none
+  | k + 1, zero => do
+    return 0
+  | k + 1, succ =>  do
+    return (Nat.succ n)
+  | k + 1, left => do
+    return n.unpair.1
+  | k + 1, right => do
+    pure n.unpair.2
+  | k + 1, oracle => do
+    -- (O n).toOption
+    -- umm. this is a contradiction. um.
+    pure (O n)
+  | k + 1, pair cf cg => do
+    Nat.pair <$> evaln' O (k + 1) cf n <*> evaln' O (k + 1) cg n
+  | k + 1, comp cf cg => do
+    let x ← evaln' O (k + 1) cg n
+    evaln' O (k + 1) cf x
+  | k + 1, prec cf cg => do
+    n.unpaired fun a n =>
+      n.casesOn (evaln' O (k + 1) cf a) fun y => do
+        let i ← evaln' O k (prec cf cg) (Nat.pair a y)
+        evaln' O (k + 1) cg (Nat.pair a (Nat.pair y i))
+  | k + 1, rfind' cf => do
+    n.unpaired fun a m => do
+      let x ← evaln' O (k + 1) cf (Nat.pair a m)
+      if x = 0 then
+        pure m
+      else
+        evaln' O k (rfind' cf) (Nat.pair a (m + 1))
+
+
+theorem evaln_eq_evaln' : evaln O s code x = evaln' O s code x := by
+  match s with
+  | 0 => unfold evaln; unfold evaln'; simp
+  | k+1 =>
+    induction code with
+    | zero => unfold evaln; unfold evaln'; simp
+    | succ => unfold evaln; unfold evaln'; simp
+    | left => unfold evaln; unfold evaln'; simp
+    | right => unfold evaln; unfold evaln'; simp
+    | oracle => unfold evaln; unfold evaln'; simp
+    | pair _ _ _ _ => expose_names; unfold evaln; unfold evaln'; simp [a_ih,a_ih_1]
+    | comp _ _ _ _ =>
+      expose_names; unfold evaln; unfold evaln';
+      -- simp [←a_ih_1]
+      simp [←a_ih]
+    | prec _ _ _ _ => expose_names; unfold evaln; unfold evaln'; simp [a_ih,a_ih_1]
+    | rfind' _ _ => expose_names; unfold evaln; unfold evaln'; simp [a_ih,a_ih_1]
+
+  -- funext s code x
+  -- unfold evaln
+  -- unfold evaln'
+  -- match s, code with
+  -- | 0, _ => sorry
+  -- | k+1, zero => sorry
+  -- sorry
+
+
 
 -- /-- `eval c_evaln_aux (x,(code,s))` = `evaln s code x` -/
 /-- `eval c_evaln_aux (anything,(x,(code,s)))` = `evaln s code x` -/
@@ -304,10 +447,30 @@ def c_evaln_aux :=
   let comp_hist := right.comp right
   let n         := c_sub.comp₂ code (c_const 5)
   let m         := c_div2.comp $ c_div2.comp n
+  let ml        := left.comp m
+  let mr        := right.comp m
 
-  let pcl := c_l_get.comp₂ comp_hist (pair x (pair (left.comp m)  s)) -- the previous computation corresponding to evaluating code m.l for s steps.
-  let pcr := c_l_get.comp₂ comp_hist (pair x (pair (right.comp m) s))
-  let pc_ml_pcr := c_l_get.comp₂ comp_hist (pair pcr (pair (left.comp m) s))
+  -- pair
+  let pc_ml_x := c_l_get.comp₂ comp_hist (x.pair (ml.pair s)) -- `[ml]ₛ(x)`
+  let pc_mr_x := c_l_get.comp₂ comp_hist (x.pair (mr.pair s)) -- `[mr]ₛ(x)`
+
+  let opt_pair :=
+    c_ifz.comp₃ pc_ml_x (c_const 0) $
+    c_ifz.comp₃ pc_mr_x (c_const 0) $
+    succ.comp (pair (c_pred.comp pc_ml_x) (c_pred.comp pc_mr_x))
+
+  -- comp: `[ml]ₛ ( [mr]ₛ(x) ) `
+  let pc_mr_xM1 := c_pred.comp pc_mr_x
+  let pc_mlmr_x_lookup := c_l_get_opt.comp₂ comp_hist (pair pc_mr_xM1 (pair mr s))
+  let pc_mlmr_x :=
+    c_ifz.comp₃ pc_mr_x (c_const 0) $
+    c_ifz.comp₃ pc_mlmr_x_lookup (c_const 0) $
+    (c_pred.comp pc_mlmr_x_lookup)
+
+  -- prec: if `x.r=n+1`, then `[mr](x.l, (x.r-1, [code](x.l, x.r-1)))` else `[ml](x.l,0)`
+
+
+    -- c_l_get.comp₂ comp_hist (pair pc_mr_x (pair (left.comp m) s))
   let pc  := c_l_get.comp₂ comp_hist (pair x (pair m              s))
   let nMod4     := c_mod.comp₂ n (c_const 4)
 
@@ -315,16 +478,18 @@ def c_evaln_aux :=
 
   (c_const 0) $
 
-  c_if_eq_te.comp₄ s     (c_const 0) (c_const 0)              $ -- if s=0, then diverge
-  c_if_eq_te.comp₄ code  (c_const 0) (c_zero_g.comp₂   sM1 x) $
-  c_if_eq_te.comp₄ code  (c_const 1) (c_succ_g.comp₂   sM1 x) $
-  c_if_eq_te.comp₄ code  (c_const 2) (c_left_g.comp₂   sM1 x) $
-  c_if_eq_te.comp₄ code  (c_const 3) (c_right_g.comp₂  sM1 x) $
-  c_if_eq_te.comp₄ code  (c_const 4) (c_oracle_g.comp₂ sM1 x) $
-  -- c_if_eq_te.comp₄ nMod4 (c_const 0) ((c_pair_g pcl pcr).comp₂ sM1 x)  $
-  c_if_eq_te.comp₄ nMod4 (c_const 0) ((c_pair_g pcl pcr).comp₂ sM1 x)  $
-  c_if_eq_te.comp₄ nMod4 (c_const 1) (comp pcl pcr)           $
-  c_if_eq_te.comp₄ nMod4 (c_const 2) (prec pcl pcr)           $
+  c_if_gt_te.comp₄ x     sM1           (c_const 0)              $ -- if ¬x≤s, then diverge
+  c_if_eq_te.comp₄ s     (c_const 0) (c_const 0)                $ -- if s=0, then diverge
+  -- c_if_eq_te.comp₄ code  (c_const 0) (c_zero_g.comp₂   sM1 x) $
+  c_if_eq_te.comp₄ code  (c_const 0) (succ.comp (zero.comp   x)) $
+  c_if_eq_te.comp₄ code  (c_const 1) (succ.comp (succ.comp   x)) $
+  c_if_eq_te.comp₄ code  (c_const 2) (succ.comp (left.comp   x)) $
+  c_if_eq_te.comp₄ code  (c_const 3) (succ.comp (right.comp  x)) $
+  c_if_eq_te.comp₄ code  (c_const 4) (succ.comp (oracle.comp x)) $
+  -- c_if_eq_te.comp₄ nMod4 (c_const 0) ((c_pair_g pc_ml_x pc_mr_x).comp₂ sM1 x)  $
+  c_if_eq_te.comp₄ nMod4 (c_const 0) (opt_pair)  $
+  c_if_eq_te.comp₄ nMod4 (c_const 1) pc_mlmr_x           $
+  c_if_eq_te.comp₄ nMod4 (c_const 2) (prec pc_ml_x pc_mr_x)           $
                                       rfind' pc
 def c_evaln := c_l_get_last.comp (c_evaln_aux.comp (pair (c_const 0) c_id))
 
@@ -354,8 +519,8 @@ theorem pair_l_gt0 {x} : x>0→(Nat.pair x y)>0 := by
   rw [h]
   simp [unpair_zero]
 
-theorem c_evaln_evp_aux_0_0_0 : eval_prim O (c_evaln) (Nat.pair 0 (Nat.pair 0 0)) = Encodable.encode (evaln O 0 (0:ℕ) 0) := by
-  simp [decodeCode, evaln] -- simp rhs
+theorem c_evaln_evp_aux_0_0_0 : eval_prim O (c_evaln) (Nat.pair 0 (Nat.pair 0 0)) = Encodable.encode (evaln' O 0 (0:ℕ) 0) := by
+  simp [decodeCode, evaln'] -- simp rhs
   rw [show Nat.pair 0 0 = 0 from rfl]
   -- unfold c_evaln; simp only [eval_prim, c_l_get_last_evp]
   -- rw [c_evaln_aux]
@@ -370,7 +535,7 @@ theorem c_evaln_evp_aux_0_0_0 : eval_prim O (c_evaln) (Nat.pair 0 (Nat.pair 0 0)
   rw [show Nat.pair 0 0 = 0 from rfl]
   simp
 
-theorem c_evaln_evp_aux_x_0_0 : eval_prim O (c_evaln) (Nat.pair (x+1) (Nat.pair 0 0)) = Encodable.encode (evaln O 0 (0:ℕ) (x+1)) := by
+theorem c_evaln_evp_aux_x_0_0 : eval_prim O (c_evaln) (Nat.pair (x+1) (Nat.pair 0 0)) = Encodable.encode (evaln' O 0 (0:ℕ) (x+1)) := by
 
   let k:=(Nat.pair (x+1) (Nat.pair 0 0))-1
   have kP1_gt_0 : Nat.pair (x+1) (Nat.pair 0 0)>0 := by
@@ -387,19 +552,22 @@ theorem c_evaln_evp_aux_x_0_0 : eval_prim O (c_evaln) (Nat.pair (x+1) (Nat.pair 
     simp [s]
     simp [x_code_s]
     simp [h0]
-  -- have hsM1 {anything hist} : eval_prim O sM1 (Nat.pair anything (Nat.pair k hist)) = s := by
-  --   simp [sM1]
-  --   simp [hs]
-  -- have hcode {anything hist} : eval_prim O code_1 (Nat.pair anything (Nat.pair k hist)) = code := by
-  --   simp [code_1]
-  --   simp [x_code_s]
-  --   simp [h0]
-  simp [hs]
-  simp [decodeCode, evaln] -- simp rhs
+  have hsM1 {anything hist} : eval_prim O sM1 (Nat.pair anything (Nat.pair k hist)) = s-1 := by
+    simp [sM1]
+    simp [hs]
+  have hx {anything hist} : eval_prim O x_1 (Nat.pair anything (Nat.pair k hist)) = x := by
+    simp [x_1]
+    simp [x_code_s]
+    simp [h0]
+  have hcode {anything hist} : eval_prim O code (Nat.pair anything (Nat.pair k hist)) = 0 := by
+    simp [code]
+    simp [x_code_s]
+    simp [h0]
+  simp [hsM1, hx, hcode, hs]
+  simp [decodeCode, evaln'] -- simp rhs
 
-  
-theorem c_evaln_evp_aux_0_np1 : eval_prim O (c_evaln) (Nat.pair x (Nat.pair (n+1) 0)) = Encodable.encode (evaln O 0 (n+1:ℕ) x) := by
-  simp [decodeCode, evaln] -- simp rhs
+theorem c_evaln_evp_aux_0_np1 : eval_prim O (c_evaln) (Nat.pair x (Nat.pair (n+1) 0)) = Encodable.encode (evaln' O 0 (n+1:ℕ) x) := by
+  simp [decodeCode, evaln'] -- simp rhs
 
 
   have h0' : (Nat.pair x (Nat.pair (n + 1) 0))>0 := by
@@ -419,14 +587,27 @@ theorem c_evaln_evp_aux_0_np1 : eval_prim O (c_evaln) (Nat.pair x (Nat.pair (n+1
     simp [s]
     simp [x_code_s]
     simp [h0]
-
+  have hx {anything hist} : eval_prim O x_1 (Nat.pair anything (Nat.pair k hist)) = x := by
+    simp [x_1]
+    simp [x_code_s]
+    simp [h0]
+  have hs {anything hist} : eval_prim O s (Nat.pair anything (Nat.pair k hist)) = 0 := by
+    simp [s]
+    simp [x_code_s]
+    simp [h0]
+  have hsM1 {anything hist} : eval_prim O sM1 (Nat.pair anything (Nat.pair k hist)) = 0 := by
+    simp [sM1]
+    simp [hs]
+  have hcode {anything hist} : eval_prim O code (Nat.pair anything (Nat.pair k hist)) = (n+1) := by
+    simp [code]
+    simp [x_code_s]
+    simp [h0]
+  
   simp
   rw [←h0]
-  simp [hs]
+  simp [hx,hsM1,hcode, hs]
 
-
-
-theorem c_evaln_evp_aux (hcode_val:code≤4) : eval_prim O (c_evaln) (Nat.pair x (Nat.pair code (s+1))) = Encodable.encode (evaln O (s+1) (code:ℕ) x) := by
+theorem c_evaln_evp_aux (hcode_val:code≤4) : eval_prim O (c_evaln) (Nat.pair x (Nat.pair code (s+1))) = Encodable.encode (evaln' O (s+1) (code:ℕ) x) := by
   -- simp [decodeCode, evaln] -- simp rhs
 
   let k:=(Nat.pair x (Nat.pair code (s+1)))-1
@@ -458,30 +639,58 @@ theorem c_evaln_evp_aux (hcode_val:code≤4) : eval_prim O (c_evaln) (Nat.pair x
     simp [x_code_s]
     simp [h0]
   match code with
-  | 0 => simp [hs, hcode, hx, hsM1, decodeCode, evaln]
-  | 1 => simp [hs, hcode, hx, hsM1, decodeCode, evaln]
-  | 2 => simp [hs, hcode, hx, hsM1, decodeCode, evaln]
-  | 3 => simp [hs, hcode, hx, hsM1, decodeCode, evaln]
-  | 4 => simp [hs, hcode, hx, hsM1, decodeCode, evaln]
+  | 0 =>
+    simp [hcode, hx, hsM1, hs, decodeCode, evaln']
+    cases Classical.em (x≤s) with
+    | inl h => simp [h, Nat.not_lt_of_le h]
+    | inr h => simp [h, gt_of_not_le h, Option.bind]
+  | 1 =>
+    simp [hcode, hx, hsM1, hs, decodeCode, evaln']
+    cases Classical.em (x≤s) with
+    | inl h => simp [h, Nat.not_lt_of_le h]
+    | inr h => simp [h, gt_of_not_le h, Option.bind]
+  | 2 =>
+    simp [hcode, hx, hsM1, hs, decodeCode, evaln']
+    cases Classical.em (x≤s) with
+    | inl h => simp [h, Nat.not_lt_of_le h]
+    | inr h => simp [h, gt_of_not_le h, Option.bind]
+  | 3 =>
+    simp [hcode, hx, hsM1, hs, decodeCode, evaln']
+    cases Classical.em (x≤s) with
+    | inl h => simp [h, Nat.not_lt_of_le h]
+    | inr h => simp [h, gt_of_not_le h, Option.bind]
+  | 4 =>
+    simp [hcode, hx, hsM1, hs, decodeCode, evaln']
+    cases Classical.em (x≤s) with
+    | inl h => simp [h, Nat.not_lt_of_le h]
+    | inr h => simp [h, gt_of_not_le h, Option.bind]
   | n+5 => simp at hcode_val
 
-
+set_option maxHeartbeats 15000
 theorem c_evaln_evp_aux_nMod4_0 :
   -- eval_prim O (c_evaln) (Nat.pair o ((n+4)+1))
   eval_prim O (c_evaln) (Nat.pair x (Nat.pair ((n+4)+1) (s+1)))
     =
   let m := n.div2.div2
-  let pcl := eval_prim O (c_evaln) (Nat.pair x (Nat.pair m.l (s+1)))
-  let pcr := eval_prim O (c_evaln) (Nat.pair x (Nat.pair m.r (s+1)))
-  let pc_ml_pcr := eval_prim O (c_evaln) (Nat.pair (eval_prim O (c_evaln) (Nat.pair x (Nat.pair m.r (s+1)))) (Nat.pair m.l (s+1)))
+  let ml        := m.l
+  let mr        := m.r
+  -- pair
+  -- let pc_ml_x := c_l_get.comp₂ comp_hist (x.pair (ml.pair s)) -- `[ml]ₛ(x)`
+  -- let pc_mr_x := c_l_get.comp₂ comp_hist (x.pair (mr.pair s)) -- `[mr]ₛ(x)`
+  let pc_ml_x := eval_prim O (c_evaln) (Nat.pair x (Nat.pair ml (s+1)))
+  let pc_mr_x := eval_prim O (c_evaln) (Nat.pair x (Nat.pair mr (s+1)))
+  let opt_pair := Encodable.encode (do guard (x≤s); Nat.pair<$>(@Denumerable.ofNat (Option ℕ)) pc_ml_x<*>(@Denumerable.ofNat (Option ℕ)) pc_mr_x)
 
-       if n%4=0 then Encodable.encode (do guard (x ≤ s); Nat.pair<$>(@Denumerable.ofNat (Option ℕ)) pcl<*>(@Denumerable.ofNat (Option ℕ)) pcr)
-  else if n%4=1 then Encodable.encode (do guard (x ≤ s); let intermediate ← ((@Denumerable.ofNat (Option ℕ)) pcr); evaln O (s + 1) cf intermediate)
-  else if n%4=2 then Encodable.encode (do guard (x ≤ s); Nat.pair<$>(@Denumerable.ofNat (Option ℕ)) pcl<*>(@Denumerable.ofNat (Option ℕ)) pcr)
-  else if n%4=3 then Encodable.encode (do guard (x ≤ s); Nat.pair<$>(@Denumerable.ofNat (Option ℕ)) pcl<*>(@Denumerable.ofNat (Option ℕ)) pcr)
-  else 0
+  -- let pc_ml_pc_mr_x := eval_prim O (c_evaln) (Nat.pair (eval_prim O (c_evaln) (Nat.pair x (Nat.pair m.r (s+1)))) (Nat.pair m.l (s+1)))
 
   
+       if n%4=0 then opt_pair
+  else if n%4=1 then Encodable.encode (do let intermediate ← ((@Denumerable.ofNat (Option ℕ)) pc_mr_x); evaln O (s + 1) cf intermediate)
+  else if n%4=2 then Encodable.encode (do Nat.pair<$>(@Denumerable.ofNat (Option ℕ)) pc_ml_x<*>(@Denumerable.ofNat (Option ℕ)) pc_mr_x)
+  else if n%4=3 then Encodable.encode (do Nat.pair<$>(@Denumerable.ofNat (Option ℕ)) pc_ml_x<*>(@Denumerable.ofNat (Option ℕ)) pc_mr_x)
+  else 0
+
+
     := by
 
   -- simp [decodeCode, evaln] -- simp rhs
@@ -536,13 +745,16 @@ theorem c_evaln_evp_aux_nMod4_0 :
     simp [hn]
     simp [m]
     simp [div2_val]
+  have hml:eval_prim O ml_1 (Nat.pair 0 (Nat.pair k (eval_prim O c_evaln_aux (Nat.pair 0 k))))=ml:=by simp [ml_1,hm,ml]
+  have hmr:eval_prim O mr_1 (Nat.pair 0 (Nat.pair k (eval_prim O c_evaln_aux (Nat.pair 0 k))))=mr:=by simp [mr_1,hm,mr]
   have hnMod4 : eval_prim O nMod4 (Nat.pair 0 (Nat.pair k (eval_prim O c_evaln_aux (Nat.pair 0 k)))) = n%4 := by
     simp [nMod4]
     simp [hn]
 
-    
-  have bounds_left_aux_1 : m.l<n+4+1 := by
+
+  have bounds_left_aux_1 : ml<n+4+1 := by
     apply lt_add_one_of_le
+    unfold ml
     unfold m
     simp [div2_val]
     exact le_add_right_of_le (Nat.le_trans (unpair_left_le (n/2/2)) (le_trans (Nat.div_le_self _ _) (Nat.div_le_self _ _)))
@@ -550,43 +762,84 @@ theorem c_evaln_evp_aux_nMod4_0 :
     apply pair_r_gt0
     apply pair_l_gt0
     exact zero_lt_succ (n + 4)
-  have bounds_left_aux_2 : Nat.pair x (Nat.pair m.l (s + 1)) < k+1 := by
+  have bounds_left_aux_2 : Nat.pair x (Nat.pair ml (s + 1)) < k+1 := by
     unfold k
     simp [Nat.sub_add_cancel bounds_aux]
     apply pair_lt_pair_right
     exact pair_lt_pair_left (s+1) bounds_left_aux_1
-  have bounds_left : Nat.pair x (Nat.pair m.l (s + 1)) ≤ k := by
+  have bounds_left : Nat.pair x (Nat.pair ml (s + 1)) ≤ k := by
     apply le_of_lt_succ bounds_left_aux_2
 
-  have bounds_right_aux_1 : m.r<n+4+1 := by
+  have bounds_right_aux_1 : mr<n+4+1 := by
     apply lt_add_one_of_le
+    unfold mr
     unfold m
     simp [div2_val]
     exact le_add_right_of_le (Nat.le_trans (unpair_right_le (n/2/2)) (le_trans (Nat.div_le_self _ _) (Nat.div_le_self _ _)))
-  have bounds_right_aux_2 : Nat.pair x (Nat.pair m.r (s + 1)) < k+1 := by
+  have bounds_right_aux_2 : Nat.pair x (Nat.pair mr (s + 1)) < k+1 := by
     unfold k
     simp [Nat.sub_add_cancel bounds_aux]
     apply pair_lt_pair_right
     exact pair_lt_pair_left (s+1) bounds_right_aux_1
-  have bounds_right : Nat.pair x (Nat.pair m.r (s + 1)) ≤ k := by
+  have bounds_right : Nat.pair x (Nat.pair mr (s + 1)) ≤ k := by
     apply le_of_lt_succ bounds_right_aux_2
-      
-  have hpcl : eval_prim O pcl_1 (Nat.pair 0 (Nat.pair k (eval_prim O c_evaln_aux (Nat.pair 0 k)))) = pcl := by
-    simp [pcl_1]
+
+  have hpc_ml_x : eval_prim O pc_ml_x_1 (Nat.pair 0 (Nat.pair k (eval_prim O c_evaln_aux (Nat.pair 0 k)))) = pc_ml_x := by
+    simp [pc_ml_x_1]
     simp [comp_hist]
-    unfold pcl
-    simp [hm, hs, hx]
+    unfold pc_ml_x
+    simp [hml, hs, hx]
 
     unfold c_evaln
     unfold c_evaln_aux
     lift_lets
     rw [c_cov_rec_evp_2 bounds_left]
     simp
-  have hpcr : eval_prim O pcr_1 (Nat.pair 0 (Nat.pair k (eval_prim O c_evaln_aux (Nat.pair 0 k)))) = pcr := by
-    simp [pcr_1]
+  have hpc_mr_x : eval_prim O pc_mr_x_1 (Nat.pair 0 (Nat.pair k (eval_prim O c_evaln_aux (Nat.pair 0 k)))) = pc_mr_x := by
+    simp [pc_mr_x_1]
     simp [comp_hist]
-    unfold pcr
-    simp [hm, hs, hx]
+    unfold pc_mr_x
+    simp [hmr, hs, hx]
+
+    unfold c_evaln
+    unfold c_evaln_aux
+    lift_lets
+    rw [c_cov_rec_evp_2 bounds_right]
+    simp
+
+  have hnat_to_opt_0 : (Denumerable.ofNat (Option ℕ) 0) = Option.none := by exact rfl
+  have hnat_to_opt_1_aux {x} (h2:¬x=0) : x=x-1+1 := by exact Eq.symm (succ_pred_eq_of_ne_zero h2)
+  have hnat_to_opt_1 {x} (h3:¬x=0) : (Denumerable.ofNat (Option ℕ) x) = Option.some (x-1) := by
+    rw (config := {occs := .pos [1]}) [hnat_to_opt_1_aux h3]
+    exact rfl
+  have hopt_pair : eval_prim O opt_pair_1 (Nat.pair 0 (Nat.pair k (eval_prim O c_evaln_aux (Nat.pair 0 k)))) = opt_pair := by
+    simp [opt_pair_1]
+    simp [hpc_ml_x]
+    simp [hpc_mr_x]
+    simp [opt_pair]
+
+    simp [Seq.seq]
+    cases Classical.em (pc_ml_x=0) with
+    | inl h => simp [h, hnat_to_opt_0]
+    | inr h =>
+      #check hnat_to_opt_1 h
+      rw [hnat_to_opt_1 h]
+      cases Classical.em (pc_mr_x=0) with
+      | inl hl => simp [hl, hnat_to_opt_0]
+      | inr hr =>
+        -- simp [h]
+        -- simp [hr]
+        rw [hnat_to_opt_1 hr]
+        simp [h,hr]
+        -- simp [hr, h2 hr]
+        -- simp [hx,hs]
+        -- simp [hl]
+      -- simp [h]
+      -- simp [h, hnat_to_opt_1 h]
+
+    unfold pc_ml_x
+    unfold pc_mr_x
+    
 
     unfold c_evaln
     unfold c_evaln_aux
@@ -595,45 +848,51 @@ theorem c_evaln_evp_aux_nMod4_0 :
     simp
 
 
-
+  simp
   have stupidrewrite : (eval_prim O
                 ((c_const 0).c_cov_rec
-                  (c_if_eq_te.comp
-                    ((s_1.pair (c_const 0)).pair
+                  (c_if_gt_te.comp
+                    ((x_1.pair sM1).pair
                       ((c_const 0).pair
                         (c_if_eq_te.comp
                           ((code.pair (c_const 0)).pair
-                            ((c_zero_g.comp (sM1.pair x_1)).pair
+                            ((succ.comp (zero.comp x_1)).pair
                               (c_if_eq_te.comp
                                 ((code.pair (c_const 1)).pair
-                                  ((c_succ_g.comp (sM1.pair x_1)).pair
+                                  ((succ.comp (succ.comp x_1)).pair
                                     (c_if_eq_te.comp
                                       ((code.pair (c_const 2)).pair
-                                        ((c_left_g.comp (sM1.pair x_1)).pair
+                                        ((succ.comp (left.comp x_1)).pair
                                           (c_if_eq_te.comp
                                             ((code.pair (c_const 3)).pair
-                                              ((c_right_g.comp (sM1.pair x_1)).pair
+                                              ((succ.comp (right.comp x_1)).pair
                                                 (c_if_eq_te.comp
                                                   ((code.pair (c_const 4)).pair
-                                                    ((c_oracle_g.comp (sM1.pair x_1)).pair
+                                                    ((succ.comp (oracle.comp x_1)).pair
                                                       (c_if_eq_te.comp
                                                         ((nMod4.pair (c_const 0)).pair
-                                                          ((pcl_1.c_pair_g pcr_1).pair
+                                                          (opt_pair.pair
                                                             (c_if_eq_te.comp
                                                               ((nMod4.pair (c_const 1)).pair
-                                                                ((pcl_1.comp pcr_1).pair
+                                                                (pc_mlmr_x.pair
                                                                   (c_if_eq_te.comp
                                                                     ((nMod4.pair (c_const 2)).pair
-                                                                      ((pcl_1.prec pcr_1).pair
+                                                                      ((pc_ml_x_1.prec pc_mr_x_1).pair
                                                                         pc.rfind'))))))))))))))))))))))))))))
                 (Nat.pair 0 k))
                 =eval_prim O c_evaln_aux (Nat.pair 0 k) := rfl
 
 
-  simp [hs, hcode, hnMod4, hx, hsM1, stupidrewrite]
+  simp [hcode, hnMod4, hx, hsM1, stupidrewrite]
 
   match h:n%4 with
-  | 0 => simp [hpcl, hpcr, hkP1]
+  | 0 =>
+    simp
+    cases Classical.em (x≤s) with
+    | inl h =>
+      simp [h, Nat.not_lt_of_le h]
+    | inr h => simp [h, gt_of_not_le h, Option.bind]
+    simp [hpc_ml_x, hpc_mr_x, hkP1]
   | 1 => sorry
   | 2 => sorry
   | 3 => sorry
@@ -647,13 +906,12 @@ theorem c_evaln_evp_aux_nMod4_0 :
 
 
   simp [h]
-  simp [hpcl, hpcr]
+  simp [hpc_ml_x, hpc_mr_x]
   simp [hk]
 
 
-
 @[simp] theorem c_evaln_evp: eval_prim O (c_evaln) (Nat.pair x (Nat.pair code s)) =
-  Encodable.encode (evaln O s code x) := by
+  Encodable.encode (evaln' O s code x) := by
   -- funext inp
   -- let x:=inp.l
   let code_s:=Nat.pair code s
@@ -675,13 +933,23 @@ theorem c_evaln_evp_aux_nMod4_0 :
 
     let code:=code_s.l
     let s:=code_s.r
-    rw [show code_s = Nat.pair code s from by simp [code,s]] 
+    rw [show code_s = Nat.pair code s from by simp [code,s]]
     simp only [pair_r, pair_l]
 
 
     match hs_val:s,hcode_val:code with
-    | 0,    0   => exact c_evaln_evp_aux_0_0
-    | 0,    n+1 => exact c_evaln_evp_aux_0_np1
+    | 0,    0   =>
+      cases x with
+      | zero => exact c_evaln_evp_aux_0_0_0
+      | succ n => exact c_evaln_evp_aux_x_0_0
+    | 0,    n+1 =>
+      unfold c_evaln; unfold c_evaln_aux
+      lift_lets
+      extract_lets
+      expose_names
+      -- exact c_evaln_evp_aux_0_np1
+      simp
+      sorry
     | sM1+1, 0   => apply c_evaln_evp_aux; decide
     | sM1+1, 1   => apply c_evaln_evp_aux; decide
     | sM1+1, 2   => apply c_evaln_evp_aux; decide
@@ -700,67 +968,89 @@ theorem c_evaln_evp_aux_nMod4_0 :
       rw [succ_eq_add_one] at hs_val
 
       have h0 : code_s=Nat.pair (n+5) (sM1+1) := by
-        
+
         rw [←hs_val]
         rw [←hcode_val]
         simp only [code,s]
         simp only [pair_lr]
 
-      let pcl := Nat.pair m.l (sM1+1)
-      have pcl_lt_cs : pcl < cs := by
-        unfold pcl; rw [h0]
+      let pc_ml_x := Nat.pair m.l (sM1+1)
+      have pc_ml_x_lt_cs : pc_ml_x < code_s := by
+        unfold pc_ml_x; rw [h0]
         exact pair_lt_pair_left (sM1 + 1) _m1
-      let pcr := Nat.pair m.r (sM1+1)
-      have pcr_lt_cs : pcr < cs := by
-        unfold pcr; rw [h0]
+      let pc_mr_x := Nat.pair m.r (sM1+1)
+      have pc_mr_x_lt_cs : pc_mr_x < code_s := by
+        unfold pc_mr_x; rw [h0]
         exact pair_lt_pair_left (sM1 + 1) _m2
 
-      stop
       rw [show n+5=(n+4)+1 from rfl]
+      -- stop
 
 
       cases hno:n.bodd with
       | false => cases hn2o:n.div2.bodd with
+        -- pair
         | false =>
           have h0: n%4=0 := nMod4_eq_0 hno hn2o
           -- simplify the rhs
           -- simp
           simp [decodeCode]
-          simp [evaln,hno, hn2o]
+          simp [evaln',hno, hn2o]
 
 
-          rw [c_evaln_evp_aux_nMod4_0 h0]
+          -- rw [c_evaln_evp_aux_nMod4_0 h0]
+          rw [c_evaln_evp_aux_nMod4_0]
+          simp [h0]
+          -- rw [c_replace_oracle_evp_aux_nMod4]
 
 
-          simp only []
-          rw [ih pcr pcr_lt_cs];
-          rw [ih pcl pcl_lt_cs];
+          -- simp only []
+          rw [ih pc_mr_x pc_mr_x_lt_cs];
+          rw [ih pc_ml_x pc_ml_x_lt_cs];
 
-          simp only [pcl, pcr, m]
+          simp only [pc_ml_x, pc_mr_x, m]
           simp
 
+        -- prec
         | true =>
           have h0: n%4=2 := nMod4_eq_2 hno hn2o
-          simp [evaln, encodeCode_evaln, decodeCode, hno, hn2o] -- simplify the rhs
+
+          -- simplify the rhs
+          -- simp
+          simp [decodeCode]
+          simp [evaln',hno, hn2o]
+
+          
+          stop
+          simp [evaln', encodeCode_evaln, decodeCode, hno, hn2o] -- simplify the rhs
           rw [c_evaln_evp_aux_nMod4_2 h0]
           simp
           constructor
-          · rw [ih m.l _m1]; simp [evaln, m]
-          · rw [ih m.r _m2]; simp [evaln, m]
+          · rw [ih m.l _m1]; simp [evaln', m]
+          · rw [ih m.r _m2]; simp [evaln', m]
 
       | true => cases hn2o:n.div2.bodd with
+        -- comp
         | false =>
           have h0: n%4=1 := nMod4_eq_1 hno hn2o
-          simp [evaln, encodeCode_evaln, decodeCode, hno, hn2o] -- simplify the rhs
+
+          -- simplify the rhs
+          -- simp
+          simp [decodeCode]
+          simp [evaln',hno, hn2o]
+
+          stop
+          simp [evaln', encodeCode_evaln, decodeCode, hno, hn2o] -- simplify the rhs
           rw [c_evaln_evp_aux_nMod4_1 h0]
           simp
           constructor
-          · rw [ih m.l _m1]; simp [evaln, m]
-          · rw [ih m.r _m2]; simp [evaln, m]
+          · rw [ih m.l _m1]; simp [evaln', m]
+          · rw [ih m.r _m2]; simp [evaln', m]
 
+        -- rfind
         | true =>
           have h0: n%4=3 := nMod4_eq_3 hno hn2o
-          simp [evaln, encodeCode_evaln, decodeCode, hno, hn2o] -- simplify the rhs
+          simp [evaln', encodeCode_evaln, decodeCode, hno, hn2o] -- simplify the rhs
           rw [c_evaln_evp_aux_nMod4_3 h0]
           simp
           rw [ih m hm]; simp [evaln, m]
